cleaned rewriting code

platform/cito/SepHints2.v
@@ -3,6 +3,8 @@ Require Import List.
 
 Set Implicit Arguments.
 
+Local Open Scope nat.
+
 Variable splittable : forall A, list A -> nat -> Prop.
 
 Definition array_to_split ls p (_ : nat) := array ls p.
@@ -11,7 +13,7 @@ Lemma replace_array_to_split : forall ls p pos, array ls p = array_to_split ls p
   eauto.
 Qed.
 
-Lemma array_split : forall ls p pos, splittable ls pos -> array_to_split ls p pos ===> array (firstn pos ls) p * array (skipn pos ls) (p ^+ $4 ^* $(pos)).
+Lemma array_split : forall ls p pos, splittable ls pos -> array_to_split ls p pos ===> array (firstn pos ls) p * array (skipn pos ls) (p ^+ $(4 * pos)).
   admit.
 Qed.
 
@@ -21,11 +23,23 @@ Lemma array_elim : forall ls p, to_elim ls -> array ls p ===> p =?> length ls.
   admit.
 Qed.
 
+Definition buf_to_split p len (_ : nat) := (p =?> len)%Sep.
+
+Definition buf_splittable (len pos : nat) := pos <= len.
+
+Lemma buf_split_bwd : forall p len pos, buf_splittable len pos -> p =?> pos * (p ^+ $(4 * pos)) =?> (len - pos) ===> buf_to_split p len pos.
+  admit.
+Qed.
+
 Definition hints_array_split : TacPackage.
   prepare array_split tt.
 Defined.
 
 Definition hints_array_elim : TacPackage.
   prepare array_elim tt.
+Defined.
+
+Definition hints_buf_split_bwd : TacPackage.
+  prepare tt buf_split_bwd.
 Defined.
 
