platform/cito/VerifCondOk.v
@@ -210,6 +210,13 @@ Section TopSection.
     evaluate hints_array_split.
     fold (@firstn W) in *.
     fold (@skipn W) in *.
+    Require Import Arith.
+
+    Lemma fold_4_mult : forall n, n + (n + (n + (n + 0))) = 4 * n.
+      intros; ring.
+    Qed.
+
+    rewrite fold_4_mult in *.
     intros.
     unfold_all.
     Hint Resolve map_length.
@@ -235,30 +242,39 @@ Section TopSection.
     unfold_all.
     erewrite CancelIL.skipn_length in *.
     rewrite H27 in *.
-    Lemma replace_it3 : forall a b, $(a) ^- $(S (S b)) = natToW (a - 2 - b).
-      admit.
+    rewrite map_length in *.
+
+    Lemma replace_it3 : forall a b, 2 <= a -> b <= a - 2 -> $(a) ^- $(S (S b)) = natToW (a - 2 - b).
+      intros; replace (a - 2 - b) with (a - (2 + b)) by omega; rewrite natToW_minus; eauto.
     Qed.
 
-    rewrite replace_it3 in *.
-    rewrite Mult.mult_0_r in *.
+    rewrite replace_it3 in * by eauto.
+    Lemma fold_4_mult_2 : 4 * 2 = 8.
+      eauto.
+    Qed.
+    
+    Lemma fold_4_mult_1 : 4 * 1 = 4.
+      eauto.
+    Qed.
+
     Lemma wplus_0 : forall w : W, w ^+ $0 = w.
       intros; rewrite wplus_comm; eapply wplus_unit.
     Qed.
-    rewrite wplus_0 in *.
-    replace (4 * 2) with 8 in * by omega.
-    Lemma replace4 : forall (a : W) b c, a ^+ $(b) ^+ $(c) = a ^+ $(b + c).
-      admit.
-    Qed.
-    rewrite replace4 in *.
-    rewrite replace4 in *.
-    rewrite map_length in *.
-    Lemma replace5 : forall n, $4 ^* $(n) = natToW (4 * n).
-      admit.
-    Qed.
 
-    rewrite replace5 in *.
+    Ltac rewrite_natToW_plus :=
+      repeat match goal with
+               | H : context [ natToW (_ + _) ] |- _ => rewrite natToW_plus in H
+               | |- context [ natToW (_ + _) ] => rewrite natToW_plus
+             end.
+
+    rewrite Mult.mult_0_r in *.
+    rewrite wplus_0 in *.
+    rewrite fold_4_mult_1 in *.
+    rewrite fold_4_mult_2 in *.
     rewrite Mult.mult_plus_distr_l in *.
-    replace (4 * 1) with 4 in * by eauto.
+    rewrite_natToW_plus.
+    repeat rewrite wplus_assoc in *.
+
     generalize dependent H6; clear_all; intros.
     hide_upd_sublist.
     set (map _ _) in *.
@@ -269,13 +285,6 @@ Section TopSection.
     unfold array in h0.
     simpl in h0.
     subst h0.
-    rewrite (@Plus.plus_comm 8) in *.
-    rewrite (@Plus.plus_comm 8) in *.
-    Lemma replace6 : forall a b, 4 * a + 4 * b + 8 = 4 * a + 8 + 4 * b.
-      admit.
-    Qed.
-
-    rewrite replace6 in *.
 
     clear_imports.
     repeat hiding ltac:(step auto_ext).
@@ -318,22 +327,28 @@ Section TopSection.
     unfold array in h0.
     simpl in h0.
     subst h0.
-    rewrite Mult.mult_0_r in *.
-    rewrite wplus_0 in *.
-    replace (4 * 2) with 8 in * by omega.
-    repeat rewrite replace4 in *.
-    rewrite Mult.mult_plus_distr_l in *.
-    replace (4 * 1) with 4 in * by eauto.
-    repeat rewrite (@Plus.plus_comm 8) in *.
-    rewrite replace6 in *.
 
-    instantiate (6 := (_, _)); simpl in *.
-    instantiate (8 := v).
     instantiate (7 := upd_sublist l0 0 x13).
-    
     subst l0.
     rewrite length_upd_sublist in *.
     rewrite length_upd_sublist in *.
+
+    rewrite Mult.mult_0_r in *.
+    rewrite wplus_0 in *.
+    try rewrite fold_4_mult_1 in *.
+    rewrite fold_4_mult_2 in *.
+    rewrite Mult.mult_plus_distr_l in *.
+    rewrite_natToW_plus.
+    set (4 * length vars) in *.
+    set (4 * length x6) in *.
+    set (Regs x Sp ^+ $8) in *.
+    replace (_ ^+ natToW (n + n0)) with (w ^+ $(n) ^+ $(n0)) by (rewrite natToW_plus; rewrite wplus_assoc; eauto).
+    unfold_all.
+    repeat rewrite wplus_assoc in *.
+
+    instantiate (6 := (_, _)); simpl in *.
+    instantiate (6 := v).
+    
     set (upd_sublist x6 _ _) in *.
     set (upd_sublist l0 _ _) in *.
     assert (length x15 = length l) by admit.
@@ -348,28 +363,9 @@ Section TopSection.
     assert (to_elim x15) by (unfold to_elim; eauto).
     hiding ltac:(step hints_array_elim).
     rewrite H32 in *.
-    set (4 * _ + _ + 4 * _) in *.
-    Lemma replace7 : forall (a : W) b c, a ^+ $(b + c) = a ^+ $(b) ^+ $(c).
-      admit.
-    Qed.
-
-    repeat rewrite replace7 in *.
-    set (Regs x Sp ^+ _) in *.
-
+    set (Regs _ _ ^+ _ ^+ _ ^+ _) in *.
     set (length l) in *.
     set (x8 - _ - _) in *.
-
-    Definition buf_to_split p len (_ : nat) := (p =?> len)%Sep.
-
-    Definition buf_splittable (len pos : nat) := pos <= len.
-
-    Lemma buf_split_bwd : forall p len pos, buf_splittable len pos -> p =?> pos * (p ^+ $(4 * pos)) =?> (len - pos) ===> buf_to_split p len pos.
-      admit.
-    Qed.
-
-    Definition hints_buf_split_bwd : TacPackage.
-      prepare tt buf_split_bwd.
-    Defined.
 
     replace (w =?> x8)%Sep with (buf_to_split w x8 2) by (unfold buf_to_split; eauto).
     assert (buf_splittable x8 2) by admit.
@@ -377,15 +373,15 @@ Section TopSection.
     post.
     hiding ltac:(step auto_ext).
 
-    replace (4 * 2) with 8 in * by omega.
-
     set (w ^+ _) in *.
     set (x8 - _) in *.
-    subst n1.
+    subst n0.
     set (length l) in *.
-    replace (w0 =?> n0)%Sep with (buf_to_split w0 n0 n1) by (unfold buf_to_split; eauto).
-    assert (buf_splittable n0 n1) by admit.
+    replace (w0 =?> n)%Sep with (buf_to_split w0 n n0) by (unfold buf_to_split; eauto).
+    assert (buf_splittable n n0) by admit.
     hiding ltac:(step hints_buf_split_bwd).
+    rewrite fold_4_mult in *.
+    hiding ltac:(step auto_ext).
 
     Focus 2.
     eauto.
